SV.v
@@ -1,0 +1,115 @@
+Set Implicit Arguments.
+From SLF Require Import LabType Fun LibSepFmap Sum.
+From SLF Require Import LibSepReference LibSepTLCbuffer Struct Unary Loops COO.
+From mathcomp Require Import ssreflect ssrfun zify.
+Hint Rewrite conseq_cons' : rew_listx.
+
+Open Scope Z_scope.
+
+
+Definition to_int (v : val) : int := 
+  match v with 
+  | val_int i => i 
+  | _ => 0
+  end.
+
+Coercion to_int : val >-> Z.
+
+Lemma to_int_if P a b : 
+  to_int (If P then a else b) = If P then a else b.
+Proof. by case: classicT. Qed.
+
+Section pure_facts.
+
+Import List.
+
+Definition sorted (l : list int) : Prop. Admitted.
+
+
+End pure_facts.
+
+Module sparse_vec.
+
+Module Export AD := WithUnary(IntDom).
+
+Notation "H1 '\\*' H2" := (hstar H1 H2)
+  (at level 42, right associativity, format "H1  \\* '//' H2") : hprop_scope.
+
+Section sparse_vec.
+
+Notation "'xind'" := ("x_ind":var) (in custom trm at level 0) : trm_scope.
+Notation "'xval'" := ("x_val":var) (in custom trm at level 0) : trm_scope.
+Notation "'yind'" := ("y_ind":var) (in custom trm at level 0) : trm_scope.
+Notation "'yval'" := ("y_val":var) (in custom trm at level 0) : trm_scope.
+Notation "'iX'" := ("iX":var) (in custom trm at level 0) : trm_scope.
+Notation "'iY'" := ("iY":var) (in custom trm at level 0) : trm_scope.
+Notation "'ans'" := ("ans":var) (in custom trm at level 0) : trm_scope.
+
+Import List.
+
+Context (xind xval yind yval : list int).
+Context (Nx Ny M : int).
+Hypothesis len_xind : length xind = Nx :> int.
+Hypothesis len_xval : length xval = Nx :> int.
+Hypothesis len_yind : length yind = Ny :> int.
+Hypothesis len_yval : length yval = Ny :> int.
+Hypothesis sorted_xind : sorted xind.
+Hypothesis sorted_yind : sorted yind.
+Hypothesis xind_leq : forall x, In x xind -> 0 <= x < M.
+Hypothesis yind_leq : forall x, In x yind -> 0 <= x < M.
+
+Definition get := coo_vec.get.
+
+Notation "'while' C '{' T '}'"  :=
+  (While C T)
+  (in custom trm at level 69,
+    C, T at level 0,
+    format "'[' while  C ']'  '{' '/   ' '[' T  '}' ']'") : trm_scope.
+
+Definition dotprod := <{
+  fun xind xval yind yval =>
+    let ans = 0 in
+    let iX = ref 0 in 
+    let iY = ref 0 in 
+    let "iXl" = iX < Nx in 
+    let "iYl" = iY < Ny in
+    let "cnd" = "iXl" && "iYl" in 
+      while "cnd" {
+        let "iXind" = xind[iX] in 
+        let "iYind" = yind[iY] in 
+        let "cnd" = "iXind" = "iYind" in 
+        if "cnd" then 
+          let "iXind" = xval[iX] in 
+          let "iYind" = yval[iY] in 
+          let "val" = "iXind" * "iYind" in
+          ans += "val";
+          ++iX;
+          ++iY
+        else 
+          let "cnd" = "iXl" < "iYl" in 
+          if "cnd" then 
+            ++iX 
+          else ++iY
+      }; ans
+}>.
+
+Lemma dotprod_spec `{Inhab D} (x_ind x_val y_ind y_val : loc) : 
+  {{ arr(x_ind, xind)⟨1, 0⟩ \* arr(y_ind, yind)⟨1, 0⟩ \*
+     arr(x_val, xval)⟨1, 0⟩ \* arr(y_val, yval)⟨1, 0⟩ \\*
+     (\*_(i <- `[0, M]) arr(x_ind, xind)⟨2, i⟩) \\*
+     (\*_(i <- `[0, M]) arr(x_val, xval)⟨2, i⟩) \\* 
+     (\*_(i <- `[0, M]) arr(y_ind, yind)⟨3, i⟩) \\*
+     (\*_(i <- `[0, M]) arr(y_val, yval)⟨3, i⟩) }}
+  [{
+    [1| ld in `{0}   => dotprod x_ind x_val y_ind y_val];
+    [2| ld in `[0,M] => get Nx ld x_ind x_val];
+    [3| ld in `[0,M] => get Ny ld y_ind y_val]
+  }]
+  {{ hv, \[hv[`1](0) = Σ_(i <- `[0,M]) (hv[`2](i) * hv[`3](i))] \* \Top}}.
+Proof.
+Admitted.
+
+
+End sparse_vec.
+
+End sparse_vec.
